Example.dfy
@@ -4,18 +4,11 @@ module Example {
   import opened Parsing
 
   method Main() {
-    var digitP := Parser<char>.Digit();
-    var letterP := Parser<char>.Letter();
-    print(digitP.Parse("5")); // Some(5)
-    /* print(digitP.Parse("X")); // None */
-    /* var digitOrLetterP := digitP.Or(letterP); */
-    /* var digitOrLetterSeqP := digitOrLetterP.ZeroOrMore(); */
+    print(Parse(Digit(), "5")); // Some(5)
+    print(Parse(Digit(), "X")); // None
+    var digitOrLetter: Parser<char> := Or(Digit(), Letter());
+    print(Parse(digitOrLetter, "X")); // Some(X)
+    print(Parse(digitOrLetter, "+")); // None
 
-    /* var idP: Parser<string> := letterP.Then(digitOrLetterSeqP, (c, cs) => [c] + cs); */
-
-    /* print(idP.Parse("x"));   // Some(x) */
-    /* print(idP.Parse("x23")); // Some(X23) */
-    /* print(idP.Parse("A_Z")); // Some(A_Z) */
-    /* print(idP.Parse("12"));  // None */
   }
 }
